Language/Parse.v
@@ -1,1 +1,311 @@
+From Coq Require Import Strings.String.
+From Coq Require Import Strings.Ascii.
+From Coq Require Import Init.Nat.
+From Coq Require Import Lists.List. Import ListNotations.
+From Language Require Import Error.
+From Language Require Import Language.
 
+Definition isWhite (c : ascii) : bool :=
+  let n := nat_of_ascii c in
+  orb (orb (n =? 32)   (* space *)
+           (n =? 9))   (* tab *)
+      (orb (n =? 10)   (* linefeed *)
+           (n =? 13)). (* Carriage return. *)
+
+Definition isLowerAlpha (c : ascii) : bool :=
+  let n := nat_of_ascii c in
+    andb (97 <=? n) (n <=? 122).
+
+Definition isAlpha (c : ascii) : bool :=
+  let n := nat_of_ascii c in
+    orb (andb (65 <=? n) (n <=? 90))
+        (andb (97 <=? n) (n <=? 122)).
+
+Definition isDigit (c : ascii) : bool :=
+  let n := nat_of_ascii c in
+     andb (48 <=? n) (n <=? 57).
+
+Inductive chartype := white | alpha | digit | other.
+
+Definition classifyChar (c : ascii) : chartype :=
+  if isWhite c then
+    white
+  else if isAlpha c then
+    alpha
+  else if isDigit c then
+    digit
+  else
+    other.
+
+Fixpoint list_of_string (s : string) : list ascii :=
+  match s with
+  | EmptyString => []
+  | String c s => c :: (list_of_string s)
+  end.
+
+Definition string_of_list (xs : list ascii) : string :=
+  fold_right String EmptyString xs.
+
+Definition token := string.
+
+(* More precise tokenizer *)
+(* 
+  - cls the chartype your are waiting for
+  - acc the accumulator for the current token
+  - xs the rest of the string (=list ascii) to parse.
+*)
+Fixpoint tokenize_helper (cls : chartype) (acc xs : list ascii)
+                       : list (list ascii) :=
+  let tk := match acc with
+          | [] => []
+          | _::_ => [acc] end in
+  match xs with
+  | [] => tk
+  | (x::xs') =>
+    match cls, classifyChar x, x with
+    | _, _, "("      =>
+      tk ++ ["("]::(tokenize_helper other [] xs')
+    | _, _, ")"      =>
+      tk ++ [")"]::(tokenize_helper other [] xs')
+    | _, white, _    =>
+      tk ++ (tokenize_helper white [] xs')
+    | alpha,alpha,x  =>
+      tokenize_helper alpha (x::acc) xs'
+    | alpha, digit, x =>
+      tokenize_helper alpha (x::acc) xs'
+    | digit,digit,x  =>
+      tokenize_helper digit (x::acc) xs'
+    | other,other,x  =>
+      tokenize_helper other (x::acc) xs'
+    | _,tp,x         =>
+      tk ++ (tokenize_helper tp [x] xs')
+    end
+  end %char.
+
+Definition tokenize (s : string) : list string :=
+  map
+    (fun l => string_of_list (rev l))
+    (tokenize_helper white [] (list_of_string s)).
+
+Module TestTokenize.
+
+Compute tokenize "let2if abcdefg123456 if let3 23 cdjnc 2a".
+Example test1 :
+    tokenize "let abc12=3;  223*(3+(a+c)) ;
+    foo(drop(x))"
+  = ["let";"abc12"; "="; "3"; ";"; "223";
+     "*"; "("; "3"; "+"; "("; "a"; "+"; "c";
+     ")"; ")"; ";"; "foo"; "("; "drop"; "(";
+     "x"; ")"; ")"]%string.
+Proof. reflexivity. Qed.
+
+Example test2 : tokenize "let x = foo ( drop(y)) y;"
+= ["let"; "x"; "=";"foo"; "("; "drop"; "("; "y";
+   ")"; ")"; "y"; ";"]%string.
+Proof. reflexivity. Qed.
+
+Compute tokenize "let x = 4;".
+
+End TestTokenize.
+
+Notation "'let+' p = e1 ; e2"
+   := (match e1 with
+       | Ok p => e2
+       | Error err => Error err
+       end)
+   (right associativity, p pattern, at level 60, e1 at next level).
+
+Notation "'try' e1 'or' e2"
+   := (
+    let result := e1 in
+    match result with
+       | Ok _  => result
+       | Error _ => e2
+       end)
+   (right associativity,
+    at level 60, e1 at next level, e2 at next level).
+
+(* TODO put this in Error.v *)
+
+(* Definition parser (T : Type) := *)
+(*   list token -> result (T * list token). *)
+
+Fixpoint many_helper {T} 
+  (p : list token -> result (T * list token)) 
+  acc steps xs :=
+  match steps, p xs with
+  | 0, _ =>
+      Error "Too many recursive calls"
+  | _, Error _ =>
+      Ok ((rev acc), xs)
+  | S steps', Ok (t, xs') =>
+      many_helper p (t :: acc) steps' xs'
+  end.
+
+(** A (step-indexed) parser that expects zero or more [p]s: *)
+
+Definition many {T}
+  (p : list token -> result (T * list token))
+  (steps : nat) : list token -> result (list T * list token) :=
+  many_helper p [] steps.
+
+(** A parser that expects a given token, followed by [p]: *)
+Definition firstExpect {T}
+  (t : token)
+  (p : list token -> result (T * list token))
+  : list token -> result (T * list token) :=
+  fun xs => match xs with
+            | x::xs' =>
+              if string_dec x t
+              then p xs'
+              else Error ("expected '" ++ t ++ "'.")
+            | [] =>
+              Error ("expected '" ++ t ++ "'.")
+            end.
+
+(** A parser that expects a particular token: *)
+Definition expect (t : token) : list token -> result (unit * list token) :=
+  firstExpect t (fun xs => Ok (tt, xs)).
+
+(* We suppose that we get token from the previous lexer *)
+Definition parseIdentifier
+  (l : list token) : result (string * list token) :=
+  match l with 
+  | [] => Error "Expected identifier"
+  | h::q => 
+      match list_of_string h with
+      | [] => Error "Empty token"
+      | c::s =>
+        if isAlpha c then
+          Ok(h, q)
+        else 
+          Error "Identifier should begin with a Letter"
+      end
+  end.
+
+Definition parseNumber (xs : list token)
+                     : result (nat * list token) :=
+match xs with
+| [] => Error "Expected number"
+| x::xs' =>
+    if forallb isDigit (list_of_string x) then
+      Ok (fold_left
+               (fun n d =>
+                  10 * n + (nat_of_ascii d -
+                            nat_of_ascii "0"%char))
+               (list_of_string x)
+               0,
+             xs')
+    else
+      Error "Expected number"
+end.
+
+Fixpoint parseSimpleExpression (steps : nat) (rest : list token)
+  : result (expression * list token) :=
+  match steps with
+  | O => Error "Too Much Steps for Parsing"
+  | S n =>
+  match rest with
+  | [] => Ok(Value UnitV, [])
+  | _::_ =>
+
+  try
+    let+ ( x, rest) = (firstExpect "let"%string parseIdentifier) rest;
+    let+ (e1, rest) = (firstExpect "="%string (parseSimpleExpression n)) rest;
+    let+ (e2, rest) = (firstExpect ";"%string (parseExpression n)) rest;
+    Ok (Let x e1 e2, rest)
+  or try
+    let+ ( x, rest) = parseIdentifier rest;
+    let+ ( e, rest) = (firstExpect "="%string (parseSimpleExpression n)) rest;
+    Ok (Assign x e, rest)
+  or try
+    let+ ( f, rest) = parseIdentifier rest;
+    let+ ( _, rest) = (expect "("%string) rest;
+    let+ ( l, rest) = (parseArguments n) rest;
+    let+ ( _, rest) = (expect ")"%string) rest;
+    Ok (FunctionCall f l, rest)
+  or try
+    let+ ( i, rest) = parseNumber rest;
+    Ok (Value (IntV i), rest)
+  or try
+    let+ ( x, rest) = parseIdentifier rest;
+    Ok (Var x, rest)
+  or try
+    let+ ( _, rest) = (expect "("%string) rest;
+    let+ ( _, rest) = (expect ")"%string) rest;
+    Ok (Value UnitV, rest)
+  or
+    Error "Not managed to parse"
+  end
+  end
+
+with parseArguments (steps : nat) (rest : list token)
+  : result (list expression * list token) :=
+  match steps with
+  | O => Error "Too Much Steps for Parsing"
+  | S n =>
+  try
+    let+ (e1, rest) = (parseExpression n) rest;
+    let+ ( l, rest) = (firstExpect ","%string (parseArguments n)) rest;
+    Ok (e1 :: l, rest)
+  or try
+    let+ (e1, rest) = (parseExpression n) rest;
+    Ok ([e1], rest)
+  or
+    let+ ( _,    _) = (expect ")"%string) rest;
+    Ok ([], rest)
+  end
+
+with parseExpression (steps : nat) (rest : list token)
+  : result (expression * list token) :=
+  match steps with
+  | O => Error "Too Much Steps for Parsing"
+  | S n =>
+  try
+    let+ (e1, rest) = (parseSimpleExpression n) rest;
+    let+ (e2, rest) = (firstExpect ";"%string (parseExpression n)) rest;
+    Ok (Sequence e1 e2, rest)
+  or
+    let+ ( e, rest) = (parseSimpleExpression n) rest;
+    Ok (e, rest)
+  end.
+
+Definition BigNat := 1000.
+
+Definition parseSimple (s : string) : result expression :=
+  match parseSimpleExpression BigNat (tokenize s) with
+  | Ok (res,  [] ) => Ok res
+  | Ok (res, _::_) => Error "Some token left to parse"
+  | Error err => Error err
+  end.
+
+Definition parse (s : string) : result expression :=
+  match parseExpression BigNat (tokenize s) with
+  | Ok (res,  [] ) => Ok res
+  | Ok (res, _::_) => Error "Some token left to parse"
+  | Error err => Error err
+  end.
+
+Module TestParse.
+Compute parse "3".
+Compute parse "x234".
+Compute parse "x = 4".
+Compute parse "x = y".
+Compute parse "let x = y;".
+Compute parse "let x = y; 3".
+Compute parse "let x = y; let z23 = 3;".
+Compute parse "let x = y; let z23 = 3". (* Error *)
+Compute parse "foo23()".
+Compute parse "foo23(x)".
+Compute parse "foo23(x, y)".
+Compute parse "let x = foo23(); 4; x = 4".
+Compute parse "let x = foo23(x, y); 4".
+Compute parse "3 ; 4".
+Compute parse "x = 3; x = 6".
+Compute parse "let x = 4;".
+Compute parse "let x = 4; x".
+Compute parse "let abc let". (* Error *)
+Compute parse "let x = 4; let y = 12 ; 23".
+Compute parse "x = 4;".
+Compute parse "let x = 4; y = 12; 23".
+End TestParse.
