Language/Error.v
@@ -1,0 +1,42 @@
+From Language Require Import Language.
+From Coq Require Import Strings.String.
+
+(* Result Type for Function that can fail *)
+Inductive result (X: Type) : Type :=
+  | Ok: X -> result X
+  (* | Ok (x : X) *)
+  | Error (s : string).
+
+(* Inductive res (A: Type) : Type := *)
+(* | OK: A -> res A *)
+(* | Error: errmsg -> res A. *)
+Arguments Ok [X].
+Arguments Error [X].
+
+(* Check Ok. *)
+
+(* Inductive result (A E: Type) : Type := *)
+(* | Ok (x : A) *)
+(* | Error (error : E). *)
+(**)
+(* Arguments Ok [A E]. *)
+(* Arguments Error [A E]. *)
+
+(* return monad TODO *)
+
+Inductive customError : Type :=
+  | ExecutionError
+  | NonTerminatingFunction
+  | Todo
+  | VariableNotTypable
+  | TypeError (expected given : type).
+
+(* Notation "let+ x = y ; e " := ( *)
+(*   match y with *)
+(*     | Ok a => let x := a in e *)
+(*     | Error err => Error err *)
+(*   end *)
+(*   ) (no associativity, only parsing, at level 50). *)
+
+Module Test.
+End Test.
