Language/Semantics.v
@@ -1,0 +1,45 @@
+From Language Require Import Language.
+From Language Require Import Parse.
+From Language Require Import Error.
+Require Import Coq.Bool.Bool.
+Require Import Coq.Strings.String.
+Local Open Scope string_scope.
+Require Import Coq.Lists.List.
+Require Import Integers.
+Import ListNotations.
+
+(*********************************
+   Relation Operational Semantics
+**********************************)
+Inductive semantics_expression : execution_state -> execution_state -> Prop :=
+  | VarSem (ex1 ex2 : execution_state) : semantics_expression ex1 ex2.
+
+Module SemanticsRelationTest.
+(* Example example50 : forall (x : variable) (tau : type), *)
+  (* (type_expression [(x, (None, tau))] x tau). *)
+(* Proof. apply Env_Empty. Qed. *)
+End SemanticsRelationTest.
+
+
+(********************************
+  Function Operational Semantics
+*********************************)
+Fixpoint semantics_expression_exec 
+  (n : nat) (ex : execution_state) : result execution_state :=
+  match n with
+  | 0 => Error "NonTerminatingFunction"
+  | S i =>
+  let (sigma, ex_stack) := ex in
+  match ex_stack with
+  | [] => Error "Todo"
+  | (env_stack, e)::ex_stack' =>
+    match e with
+    | _ => Error "Todo"
+    end
+      (* semantics_expression_exec i (sigma, ex_stack') *)
+  end
+  end.
+
+(* Example example250 : forall (x : variable), *)
+  (* semantics_expression_exec BigNat []. *)
+
