Language/Typing.v
@@ -1,0 +1,124 @@
+From Language Require Import Language.
+From Language Require Import Parse.
+From Language Require Import Error.
+Require Import Coq.Bool.Bool.
+Require Import Coq.Strings.String.
+Local Open Scope string_scope.
+Require Import Coq.Lists.List.
+Require Import Integers.
+Import ListNotations.
+
+(****************************
+   Relation Typing Expression
+ *****************************)
+
+Inductive type_expression : typingEnv -> expression -> type -> typingEnv 
+  -> Prop :=
+  | VarType (x : variable) (tau : type) :
+    type_expression [(x, (None, tau))] (Var x) tau [(x, (None, tau))]
+  | Env_Rec (gamma : typingEnv) (x y : variable) (taux tauy : type) :
+      x <> y
+      -> type_expression ((y, (None, tauy))::gamma) (Var x) taux
+        ((y, (None, tauy))::gamma)
+      -> type_expression gamma (Var x) taux gamma.
+Example example100 : forall (x : variable) (tau : type),
+  type_expression [(x, (None, tau))] (Var x) tau [(x, (None, tau))].
+Proof. apply VarType. Qed.
+
+(***************************
+  Function Typing Variable
+***************************)
+Fixpoint type_var_exec
+  (gamma : typingEnv) (x : variable) : (result (type * typingEnv)) :=
+    match gamma with
+    | [] => Error ("Variable " ++ x ++ " Not Typable")
+    | (y , (_, tau))::gamma' =>
+        if (String.eqb x y)
+        then
+          match tau with
+          | UnitT | BoolT | IntT => Ok (tau, gamma)
+          | StringT => Ok (tau, (y, (NotAccessible, tau))::gamma')
+          end
+        else (type_var_exec gamma' x)
+  end.
+
+Module TypingVarExample.
+Example example150 : forall (x : variable),
+  type_var_exec [] x = Error "Variable NotTypable".
+Proof. reflexivity. Qed.
+Example example151 : forall (x y : variable),
+  Nat.eqb x y = true ->
+  type_var_exec [(y, (None, Int))] x = Ok (Int, [(y, (None, Int))]).
+Proof. intros. simpl. rewrite H. reflexivity. Qed.
+Example example152 : forall (x : variable),
+  type_var_exec [] x = Error VariableNotTypable.
+Proof. reflexivity. Qed.
+End TypingVarExample.
+
+(*****************************
+  Function Typing Expression
+*****************************)
+Fixpoint type_expression_exec
+  (n : nat) (gamma : typingEnv) (e : expression)
+  : (result (type * typingEnv) customError) :=
+  match n with
+  | 0 => Error NonTerminatingFunction
+  | S i =>
+  match e with
+  | Sequence e1 e2 =>
+      match type_expression_exec i gamma e1 with
+      | Error err => Error err
+      | Ok (tau1, gamma1) =>
+          match type_expression_exec i gamma1 e2 with
+          | Error err => Error err
+          | Ok (tau2, gamma2) =>
+              if (type_eqb tau1 Unit)
+              then Ok (tau2, gamma2)
+              else Error (TypeError Unit tau1)
+          end
+      end
+  | Let x e1 e2 =>
+      match type_expression_exec i gamma e1 with
+      | Ok (tau1, gamma1) =>
+          type_expression_exec i ((x, (None, tau1))::gamma1) e2
+      | err => err
+      end
+  | Var x =>
+    match type_var_exec gamma x with
+    | Error err => Error err
+    | Ok (tau, gamma') => Ok (tau, gamma') (* TODO get different gamma borrow checking *)
+    end
+  | Value v => Ok (value_to_type v, gamma)
+  | Assign x e =>
+    match type_expression_exec i gamma e with
+    | Error err => Error err
+    | Ok (tau, gamma') => Error Todo
+    end
+  | _ => Error Todo
+  end
+  end.
+
+(* BigInt use for making sure function terminates *)
+Definition BigNat := 1000.
+(* Check BigNat. *)
+
+Example example200 : forall (x : variable),
+  type_expression_exec BigNat [] (Value (IntValue 4128)) = Ok (Int, []).
+  (* 4128 : int *)
+Proof. intros. reflexivity. Qed.
+Example example201 : forall (x : variable),
+  type_expression_exec BigNat []
+  (Let x (Value (IntValue 4128)) (Var x))
+  (* let x = 4128; x : int *)
+    = Ok (Int, [(x, (None, Int))]).
+Proof. intros. simpl. Search "eqb_refl". rewrite Nat.eqb_refl. reflexivity. Qed.
+Example example202 : forall (x : variable) (s : nat),
+  type_expression_exec BigNat [] 
+  (Let x (Value (StringValue s)) (Var x))
+  (* let x = s; x *)
+    = Ok (String, [(x, (NotAccessible, String))]).
+Proof. intros. simpl. rewrite Nat.eqb_refl. reflexivity. Qed.
+
+Compute type_expression_exec BigNat [] 
+  (Let 0 (Value (StringValue 1)) (Var 0)).
+
